src/StatDb/StatDbAPI.v
@@ -1,0 +1,44 @@
+Require Import POCS.
+
+
+Definition State := list nat.
+
+Definition add_spec v : Specification unit unit unit State :=
+  fun (_ : unit) state => {|
+    pre := True;
+    post := fun r state' =>
+      r = tt /\ state' = v :: state;
+    recover := fun _ _ => False
+  |}.
+
+Definition mean_spec : Specification unit (option nat) unit State :=
+  fun (_ : unit) state => {|
+    pre := True;
+    post := fun r state' =>
+      state' = state /\
+      (state = nil /\ r = None \/
+       state <> nil /\ r = Some (fold_right plus 0 state / length state));
+    recover := fun _ _ => False
+  |}.
+
+Definition wipe (state state' : State) := False.
+
+
+Module Type StatDbAPI.
+
+  Parameter init : prog InitResult.
+  Parameter add : nat -> prog unit.
+  Parameter mean : prog (option nat).
+  Parameter recover : prog unit.
+
+  Parameter abstr : Abstraction State.
+
+  Axiom add_ok : forall v, prog_spec (add_spec v) (add v) recover abstr.
+  Axiom mean_ok : prog_spec mean_spec mean recover abstr.
+  Axiom recover_noop : rec_noop recover abstr wipe.
+
+  Hint Resolve add_ok.
+  Hint Resolve mean_ok.
+  Hint Resolve recover_noop.
+
+End StatDbAPI.
