src/Variables/VariablesAPI.v
@@ -1,66 +1,57 @@
 Require Import POCS.
 
-Module Vars.
 
-  Inductive var :=
-  | VarCount
-  | VarSum.
+Inductive var :=
+| VarCount
+| VarSum.
 
-  Axiom init : prog InitResult.
-  Axiom read : var -> prog nat.
-  Axiom write : var -> nat -> prog unit.
-  Axiom var_recover : prog unit.
+Record State := mkState {
+  StateCount : nat;
+  StateSum : nat;
+}.
+
+Definition read_spec v : Specification _ _ unit _ :=
+  fun '(count, sum) state => {|
+    pre := StateCount state = count /\ StateSum state = sum;
+    post := fun r state' =>
+      state' = state /\
+      match v with
+      | VarCount => r = count
+      | VarSum => r = sum
+      end;
+    recover := fun _ _ => False
+  |}.
+
+Definition write_spec v val : Specification _ _ unit _ :=
+  fun '(count, sum) state => {|
+    pre := StateCount state = count /\ StateSum state = sum;
+    post := fun r state' =>
+      r = tt /\
+      match v with
+      | VarCount => state' = mkState val sum
+      | VarSum => state' = mkState count val
+      end;
+    recover := fun _ _ => False
+  |}.
+
+Definition wipe (state state' : State) := False.
 
 
-  (** The state the program manipulates as it executes. *)
-  Record State := mkState {
-    StateCount : nat;
-    StateSum : nat;
-  }.
+Module Type VarsAPI.
+
+  Parameter init : prog InitResult.
+  Parameter read : var -> prog nat.
+  Parameter write : var -> nat -> prog unit.
+  Parameter recover : prog unit.
 
   Axiom abstr : Abstraction State.
 
+  Axiom read_ok : forall v, prog_spec (read_spec v) (read v) recover abstr.
+  Axiom write_ok : forall v val, prog_spec (write_spec v val) (write v val) recover abstr.
+  Axiom recover_noop : rec_noop recover abstr wipe.
 
-  Axiom read_ok : forall v,
-    prog_spec
-      (fun '(count, sum) state => {|
-        pre := StateCount state = count /\ StateSum state = sum;
-        post := fun r state' =>
-          state' = state /\
-          match v with
-          | VarCount => r = count
-          | VarSum => r = sum
-          end;
-        recover := fun _ _ => False
-      |})
-      (read v) var_recover abstr.
   Hint Resolve read_ok.
-
-  Axiom write_ok : forall v val,
-    prog_spec
-      (fun '(count, sum) state => {|
-        pre := StateCount state = count /\ StateSum state = sum;
-        post := fun r state' =>
-          r = tt /\
-          match v with
-          | VarCount => state' = mkState val sum
-          | VarSum => state' = mkState count val
-          end;
-        recover := fun _ _ => False
-      |})
-      (write v val) var_recover abstr.
   Hint Resolve write_ok.
-
-
-  Definition wipe (state state' : State) := False.
-
-  Axiom recover_noop : rec_noop var_recover abstr wipe.
   Hint Resolve recover_noop.
 
-End Vars.
-
-Extraction Language Haskell.
-
-Extract Constant Vars.read => "Variables.read".
-Extract Constant Vars.write => "Variables.write".
-Extract Constant Vars.abstr => "Hoare.Build_LayerAbstraction".
+End VarsAPI.
