src/Variables/VariablesImpl.v
@@ -1,0 +1,23 @@
+Require Import POCS.
+Require Import VariablesAPI.
+
+
+Extraction Language Haskell.
+
+Module Vars <: VarsAPI.
+
+  Axiom init : prog InitResult.
+  Axiom read : var -> prog nat.
+  Axiom write : var -> nat -> prog unit.
+  Axiom recover : prog unit.
+
+  Axiom abstr : Abstraction State.
+
+  Axiom read_ok : forall v, prog_spec (read_spec v) (read v) recover abstr.
+  Axiom write_ok : forall v val, prog_spec (write_spec v val) (write v val) recover abstr.
+  Axiom recover_noop : rec_noop recover abstr wipe.
+
+End Vars.
+
+Extract Constant Vars.read => "Variables.read".
+Extract Constant Vars.write => "Variables.write".
